Retarget Pledge library over unobservable

pulse/share/steel/examples/pulse/lib/pledge/Pulse.Lib.Par.Pledge.Simple.fst
@@ -24,52 +24,6 @@ module P = Pulse.Lib.Par.Pledge
 let pledge (f:vprop) (v:vprop) : vprop =
   P.pledge_any f v
 
-(* helpers, repeated from Pulse.Lib.Par.Pledge *)
-let comm_pre (#a:Type0) (#o:inames) (#pre1 #pre2 : vprop) (#post : a -> vprop)
-  (f : stt_ghost a o (pre1 ** pre2) post)
-     : stt_ghost a o (pre2 ** pre1) post
-=
-  sub_stt_ghost _ _ (vprop_equiv_comm _ _)
-                    (intro_vprop_post_equiv _ _ (fun _ -> vprop_equiv_refl _))
-                     f
-
-let comm_post (#a:Type0) (#o:inames) (#pre : vprop) (#post1 #post2 : a -> vprop)
-  (f : stt_ghost a o pre (fun x -> post1 x ** post2 x))
-     : stt_ghost a o pre (fun x -> post2 x ** post1 x)
-=
-  sub_stt_ghost _ _ (vprop_equiv_refl _)
-                    (intro_vprop_post_equiv _ _ (fun _ -> vprop_equiv_comm _ _))
-                     f
-
-(* sigh *)
-let assoc_l_pre (#t:Type0) (#o:inames) (#a #b #c : vprop) (#post : t -> vprop)
-  (f : stt_ghost t o (a ** (b ** c)) post)
-     : stt_ghost t o ((a ** b) ** c) post
-=
-  sub_stt_ghost _ _ (vprop_equiv_sym _ _ (vprop_equiv_assoc _ _ _))
-                    (intro_vprop_post_equiv _ _ (fun _ -> vprop_equiv_refl _))
-                     f
-
-inline_for_extraction
-val frame_stt_ghost_left
-  (#a:Type0)
-  (#opens:inames)
-  (#pre:vprop) (#post:a -> vprop)
-  (frame:vprop)
-  (e:stt_ghost a opens pre post)
-  : stt_ghost a opens (frame ** pre) (fun x -> frame ** post x)
-let frame_stt_ghost_left #a #opens #pre #post frame e =
-  let e : stt_ghost a opens (pre ** frame) (fun x -> post x ** frame) =
-    frame_stt_ghost frame e
-  in
-  let e : stt_ghost a opens (frame ** pre) (fun x -> post x ** frame) =
-    comm_pre e
-  in
-  let e : stt_ghost a opens (frame ** pre) (fun x -> frame ** post x) =
-    comm_post e
-  in
-  e
-
 (* Anything that holds now holds in the future too. *)
 ```pulse
 ghost
@@ -87,7 +41,7 @@ let return_pledge = __return_pledge
 ```pulse
 ghost
 fn __make_pledge (#os:inames) (f v extra : vprop)
-               (k : (unit -> stt_ghost unit os (f ** extra) (fun _ -> f ** v)))
+               (k : ustep os (f ** extra) (f ** v))
   requires extra
   ensures pledge f v
 {
@@ -122,10 +76,27 @@ fn __redeem_pledge (f v : vprop)
 let redeem_pledge = __redeem_pledge
 
 ```pulse
+unobservable
+fn __bind_pledge_simple_aux (#f #v1 #v2 : vprop)
+       (extra : vprop)
+       (invs : inames)
+       (k : (unit -> stt_unobservable unit invs (f ** extra ** v1) (fun _ -> f ** P.pledge invs f v2)))
+       (_:unit)
+       requires f ** extra ** v1
+       ensures f ** P.pledge invs f v2
+       opens invs
+{
+  k ();
+}
+```
+
+#set-options "--log_failing_queries --split_queries always --print_implicits --print_full_names"
+
+```pulse
 ghost
 fn __bind_pledge (#os : inames) (#f #v1 #v2 : vprop)
        (extra : vprop)
-       (k : (unit -> stt_ghost unit os (f ** extra ** v1) (fun () -> f ** pledge f v2)))
+       (k : ustep os (f ** extra ** v1) (f ** pledge f v2))
    requires pledge f v1 ** extra
     ensures pledge f v2
 {
@@ -135,11 +106,13 @@ fn __bind_pledge (#os : inames) (#f #v1 #v2 : vprop)
   
   let invs = join_inames is os;
   pledge_sub_inv is invs f v1;
-  assert (P.pledge invs f v1);
+  assert (P.pledge invs f v1 ** extra);
   
-  (* This is just a subtyping of `k`. Once lambdas land this should
-  be easy to write. *)
-  let k' : (unit -> stt_ghost unit invs (f ** extra ** v1) (fun () -> f ** P.pledge invs f v2)) =
+  let k' : (unit -> stt_unobservable unit invs (f ** extra ** v1) (fun _ -> f ** P.pledge invs f v2)) =
+    (* FIXME: It's actually unclear if we can define this, since we
+       would have to know the invariants that second pledge would use,
+       but nothing prevents them from depending on whenever the function
+       is called (i.e. classical order of quantifiers problem.) *)
     admit();
   
   P.bind_pledge #invs #f #v1 #v2 extra k';
@@ -154,11 +127,19 @@ let bind_pledge #os #f #v1 #v2 extra k = __bind_pledge #os #f #v1 #v2 extra k
 ghost
 fn __bind_pledge' (#os : inames) (#f #v1 #v2 : vprop)
        (extra : vprop)
-       (k : (unit -> stt_ghost unit os (extra ** v1) (fun () -> pledge f v2)))
+       (k : (unit -> stt_unobservable unit os (extra ** v1) (fun () -> pledge f v2)))
    requires pledge f v1 ** extra
     ensures pledge f v2
 {
-  bind_pledge #os #f #v1 #v2 extra (fun () -> assoc_l_pre (frame_stt_ghost_left f (k ())))
+  unobservable fn
+  framed (_:unit)
+    requires f ** extra ** v1
+    ensures f ** pledge f v2
+    opens os
+  {
+    k ();
+  };
+  bind_pledge #os #f #v1 #v2 extra framed;
 }
 ```
 let bind_pledge' = __bind_pledge'
@@ -191,7 +172,7 @@ fn __join_pledge (#f v1 v2 : vprop)
 let join_pledge = __join_pledge
 
 ```pulse
-ghost
+unobservable
 fn __split_pledge (#f v1 v2 : vprop)
   requires pledge f (v1 ** v2)
   ensures pledge f v1 ** pledge f v2
@@ -214,7 +195,7 @@ let split_pledge = __split_pledge
 ```pulse
 ghost
 fn __rewrite_pledge (#os : inames) (#f : vprop) (v1 v2 : vprop)
-   (k : (unit -> stt_ghost unit os v1 (fun _ -> v2)))
+   (k : ustep os v1 v2)
    requires pledge f v1
     ensures pledge f v2
 {
@@ -226,10 +207,15 @@ fn __rewrite_pledge (#os : inames) (#f : vprop) (v1 v2 : vprop)
   
   pledge_sub_inv is invs f v1;
 
-  (* Again: This is just a subtyping of `k`. Once lambdas land this should
-  be easy to write. *)
-  let k' : (unit -> stt_ghost unit invs v1 (fun () -> v2)) =
-    admit();
+  unobservable fn
+  k' (_:unit)
+    requires v1
+    ensures v2
+    opens invs
+  {
+    k ();
+  };
+    
   P.rewrite_pledge #invs #f v1 v2 k';
 
   fold P.pledge_any;
