pulse/share/steel/examples/pulse/lib/pledge/Pulse.Lib.Par.Pledge.fst
@@ -17,20 +17,25 @@
 module Pulse.Lib.Par.Pledge
 
 open Pulse.Lib.Pervasives
-open Pulse.Lib.Stick
+open Pulse.Lib.Trade
+
+assume
+val unobservable_reveal_bool
+    (b : erased bool)
+: stt_unobservable bool emp_inames emp (fun b' -> pure (reveal b == b'))
 
 (* A pledge is just a magic stick that preserves the antecedent. *)
 (* TODO: can this really be a ghost step? would we ever need to allocate invariants
 to redeem? We only need to allocate in split_pledge so far, but that's an operation
 that happens outside of the internal ghost step. *)
-let pledge opens f v = (@==>) #opens f (f ** v)
+let pledge opens f v = (==>*) #opens f (f ** v)
 
 let pledge_sub_inv (os1:inames) (os2:inames{inames_subset os1 os2}) (f:vprop) (v:vprop)
   : stt_ghost unit emp_inames (pledge os1 f v) (fun _ -> pledge os2 f v)
-  = stick_sub_inv _ _
+  = trade_sub_inv _ _
 
 ```pulse
-ghost
+unobservable
 fn return_pledge_aux (os:inames) (f v : vprop) ()
     requires (v ** f)
     ensures (f ** v)
@@ -44,17 +49,17 @@ fn __return_pledge (os:inames) (f v : vprop)
   requires v
   ensures pledge os f v
 {
-  intro_stick #os f (f ** v) v (return_pledge_aux os f v);
-  fold ((@==>) #os f (f ** v));
+  intro_trade #os f (f ** v) v (return_pledge_aux os f v);
+  fold ((==>*) #os f (f ** v));
   fold pledge;
 }
 ```
 let return_pledge = __return_pledge
 
 ```pulse
-ghost
+unobservable
 fn make_pledge_aux (os:inames) (f v extra : vprop)
-                 (k : (unit -> stt_ghost unit os (f ** extra) (fun _ -> f ** v)))
+                 (k : ustep os (f ** extra) (f ** v))
                  ()
     requires extra ** f
     ensures f ** v
@@ -67,37 +72,37 @@ fn make_pledge_aux (os:inames) (f v extra : vprop)
 ```pulse
 ghost
 fn __make_pledge (os:inames) (f v extra : vprop)
-                 (k : (unit -> stt_ghost unit os (f ** extra) (fun _ -> f ** v)))
+                 (k : ustep os (f ** extra) (f ** v))
   requires extra
   ensures pledge os f v
 {
-  intro_stick #os f (f ** v) extra (make_pledge_aux os f v extra k);
-  fold ((@==>) #os f (f ** v));
+  intro_trade #os f (f ** v) extra (make_pledge_aux os f v extra k);
+  fold ((==>*) #os f (f ** v));
   fold pledge;
 }
 ```
 let make_pledge os f v extra k = __make_pledge os f v extra k
 
 ```pulse
-ghost
+unobservable
 fn __redeem_pledge (os : inames) (f v : vprop)
   requires f ** pledge os f v
   ensures f ** v
   opens os
 {
   unfold pledge;
-  unfold ((@==>) #os f (f ** v));
-  elim_stick #os f (f ** v);
+  unfold ((==>*) #os f (f ** v));
+  elim_trade #os f (f ** v);
 }
 ```
 let redeem_pledge = __redeem_pledge
 
 ```pulse
-ghost
+unobservable
 fn bind_pledge_aux
   (os : inames)
   (f v1 v2 extra : vprop)
-  (k : (unit -> stt_ghost unit os (f ** extra ** v1) (fun _ -> f ** pledge os f v2)))
+  (k : ustep os (f ** extra ** v1) (f ** pledge os f v2))
   ()
   requires f  ** (extra ** pledge os f v1)
   ensures f ** v2
@@ -118,7 +123,7 @@ fn __bind_pledge
   (#os : inames)
   (#f #v1 #v2 : vprop)
   (extra : vprop)
-  (k : (unit -> stt_ghost unit os (f ** extra ** v1) (fun _ -> f ** pledge os f v2)))
+  (k : ustep os (f ** extra ** v1) (f ** pledge os f v2))
   requires pledge os f v1 ** extra
   ensures pledge os f v2
 {
@@ -129,12 +134,12 @@ let bind_pledge #os #f #v1 #v2 extra k = __bind_pledge #os #f #v1 #v2 extra k
 
 ```pulse
 // just frames f to the left
-ghost
+unobservable
 fn __bind_pledge'_aux
   (os : inames)
   (f v1 v2 : vprop)
   (extra : vprop)
-  (k : (unit -> stt_ghost unit os (extra ** v1) (fun _ -> pledge os f v2)))
+  (k : ustep os (extra ** v1) (pledge os f v2))
   ()
   requires f ** extra ** v1
   ensures f ** pledge os f v2
@@ -150,7 +155,7 @@ fn __bind_pledge'
   (#os : inames)
   (#f #v1 #v2 : vprop)
   (extra : vprop)
-  (k : (unit -> stt_ghost unit os (extra ** v1) (fun _ -> pledge os f v2)))
+  (k : ustep os (extra ** v1) (pledge os f v2))
   requires pledge os f v1 ** extra
   ensures pledge os f v2
 {
@@ -160,7 +165,7 @@ fn __bind_pledge'
 let bind_pledge' = __bind_pledge'
 
 ```pulse
-ghost
+unobservable
 fn __join_pledge_aux (os:inames) (f v1 v2 : vprop) ()
   requires f ** (pledge os f v1 ** pledge os f v2)
   ensures f ** (v1 ** v2)
@@ -200,33 +205,32 @@ let inv_p (os0 : inames) (f v1 v2 : vprop) (r1 r2 : GR.ref bool) : vprop =
   exists* b1 b2. inv_p' os0 f v1 v2 r1 r2 b1 b2
 
 ```pulse
-atomic
-fn __elim_l_atomic (#os0:inames) (#f:vprop) (v1:vprop) (v2:vprop) (r1 r2 : GR.ref bool) (i : inv (inv_p os0 f v1 v2 r1 r2)) ()
-  requires f ** GR.pts_to r1 #one_half false ** pure (not (mem_inv os0 i))
+unobservable
+fn __elim_l (#os0:inames) (#f:vprop) (v1:vprop) (v2:vprop) (r1 r2 : GR.ref bool)
+            (i : inv (inv_p os0 f v1 v2 r1 r2){not (mem_inv os0 i)})
+            ()
+  requires f ** GR.pts_to r1 #one_half false
   ensures f ** v1
   opens (add_inv os0 i)
 {
   open Pulse.Lib.GhostReference;
-  with_invariants i {
-    ghost
+  with_invariants (i <: inv _) {
+    unobservable
     fn thunk ()
     requires f ** GR.pts_to r1 #one_half false ** inv_p os0 f v1 v2 r1 r2
     ensures (f ** v1 ** inv_p os0 f v1 v2 r1 r2)
     opens os0
     {
       unfold inv_p;
-      with bb1 bb2.
-        assert (inv_p' os0 f v1 v2 r1 r2 bb1 bb2);
       unfold inv_p';
+
+      gather2 r1;
+
       let b1 = !r1;
       let b2 = !r2;
 
-      assert (pure (b1 == bb1));
-      assert (pure (b2 == bb2));
-
-      gather2 r1;
-      let b1 : bool = stt_ghost_reveal _ b1;
-      let b2 : bool = stt_ghost_reveal _ b2;
+      let b1 : bool = unobservable_reveal_bool b1;
+      let b2 : bool = unobservable_reveal_bool b2;
 
       if b2 {
         (* The "easy" case: the big pledge has already been claimed
@@ -244,8 +248,8 @@ fn __elim_l_atomic (#os0:inames) (#f:vprop) (v1:vprop) (v2:vprop) (r1 r2 : GR.re
                   | true, false -> v2
                   | true, true -> emp) ** v1;
 
-        (* I don't understand why this remains in the ctx, but get rid
-        of it as it's just emp *)
+        (* This should just disappear when we start normalizing
+        the context. *)
         rewrite (match true, true with
                   | false, false -> pledge os0 f (v1 ** v2)
                   | false, true -> v1
@@ -255,7 +259,7 @@ fn __elim_l_atomic (#os0:inames) (#f:vprop) (v1:vprop) (v2:vprop) (r1 r2 : GR.re
 
         share2 #_ r1;
         fold (inv_p' os0 f v1 v2 r1 r2 true true);
-        fold (inv_p os0 f v1 v2 r1 r2);
+        fold inv_p;
         assert (f ** v1 ** inv_p os0 f v1 v2 r1 r2);
         drop_ (pts_to r1 #one_half true);
       } else {
@@ -272,8 +276,6 @@ fn __elim_l_atomic (#os0:inames) (#f:vprop) (v1:vprop) (v2:vprop) (r1 r2 : GR.re
 
         redeem_pledge os0 f (v1 ** v2);
 
-        assert (f ** v1 ** v2);
-
         r1 := true;
 
         rewrite v2
@@ -288,8 +290,7 @@ fn __elim_l_atomic (#os0:inames) (#f:vprop) (v1:vprop) (v2:vprop) (r1 r2 : GR.re
         fold (inv_p' os0 f v1 v2 r1 r2 true false);
         fold inv_p;
         assert (f ** v1 ** inv_p os0 f v1 v2 r1 r2);
-        drop_ (pts_to r1 #one_half true);
-        ()
+        drop_ (pts_to r1 #one_half true)
       }
     };
     thunk ()
@@ -298,37 +299,22 @@ fn __elim_l_atomic (#os0:inames) (#f:vprop) (v1:vprop) (v2:vprop) (r1 r2 : GR.re
 ```
 
 ```pulse
-ghost
-fn __elim_l (#os0:inames) (#f:vprop) (v1:vprop) (v2:vprop) (r1 r2 : GR.ref bool) (i : inv (inv_p os0 f v1 v2 r1 r2)) ()
-  requires f ** GR.pts_to r1 #one_half false
-  ensures f ** v1
-  opens (add_inv os0 i)
-{
-  admit()
-}
-```
-
-```pulse
-ghost
+unobservable
 fn __elim_r (#os0:inames) (#f:vprop) (v1:vprop) (v2:vprop) (r1 r2 : GR.ref bool) (i : inv (inv_p os0 f v1 v2 r1 r2)) ()
   requires f ** GR.pts_to r2 #one_half false
   ensures f ** v2
   opens (add_inv os0 i)
 {
+  (* Idem __elim_l *)
   admit ()
 }
 ```
 
-(* bogus.. this is an unobservable step, not ghost. Need to add support
-for unobservable in the checker. *)
-assume
-val new_invariant_ghost (p:vprop) : stt_ghost (inv p) emp_inames p (fun _ -> emp)
-
 ```pulse
-ghost
+unobservable
 fn __split_pledge (#os:inames) (#f:vprop) (v1:vprop) (v2:vprop)
   requires pledge os f (v1 ** v2)
-  returns i:iname
+  returns i:(erased iname)
   ensures pledge (add_iname os i) f v1 ** pledge (add_iname os i) f v2
 {
    let r1 = GR.alloc false;
@@ -336,26 +322,13 @@ fn __split_pledge (#os:inames) (#f:vprop) (v1:vprop) (v2:vprop)
    GR.share2 r1;
    GR.share2 r2;
 
-   rewrite (pledge os f (v1 ** v2))
-        as (match false, false with
-            | false, false -> pledge os f (v1 ** v2)
-            | false, true -> v1
-            | true, false -> v2
-            | true, true -> emp);
-
-  assert (
-     GR.pts_to r1 #one_half false
-  ** GR.pts_to r2 #one_half false
-  ** (match false, false with
-      | false, false -> pledge os f (v1 ** v2)
-      | false, true -> v1
-      | true, false -> v2
-      | true, true -> emp));
-
   fold (inv_p' os f v1 v2 r1 r2 false false);
   fold inv_p;
 
-  let i = new_invariant_ghost (inv_p os f v1 v2 r1 r2);
+  let i = new_invariant (inv_p os f v1 v2 r1 r2);
+
+  // FIXME: should follow from freshness
+  assume_ (pure (not (mem_inv os i)));
 
   make_pledge
     (add_inv os i)
@@ -371,12 +344,12 @@ fn __split_pledge (#os:inames) (#f:vprop) (v1:vprop) (v2:vprop)
     (GR.pts_to r2 #one_half false)
     (__elim_r #os #f v1 v2 r1 r2 i);
 
-  let iname = name_of_inv i;
-  
-  rewrite (pledge (add_inv os i) f v1)
-       as (pledge (add_iname os iname) f v1);
-  rewrite (pledge (add_inv os i) f v2)
-       as (pledge (add_iname os iname) f v2);
+  let iname = hide (name_of_inv i);
+
+  rewrite each
+    add_inv os i
+  as
+    add_iname os iname;
   
   iname
 }
@@ -386,9 +359,9 @@ let split_pledge = __split_pledge
 (* /split_pledge *)
 
 ```pulse
-ghost
+unobservable
 fn __rewrite_pledge_aux (os:inames) (f v1 v2 : vprop)
-      (k : (unit -> stt_ghost unit os v1 (fun _ -> v2)))
+      (k : ustep os v1 v2)
       ()
   requires (f ** emp) ** v1
   ensures  f ** pledge os f v2
@@ -402,7 +375,7 @@ fn __rewrite_pledge_aux (os:inames) (f v1 v2 : vprop)
 ```pulse
 ghost
 fn __rewrite_pledge (#os:inames) (#f v1 v2 : vprop)
-      (k : (unit -> stt_ghost unit os v1 (fun _ -> v2)))
+      (k : ustep os v1 v2)
   requires pledge os f v1
   ensures  pledge os f v2
 {
